KV get_ok and put_ok theorems. Not proven (and probably not correct!)

src/KV.v
@@ -9,6 +9,7 @@ Require Import Arith.
 Require Import Omega.
 Require Import Array.
 Require Import Psatz.
+Require Import MemLog.
 
 Import ListNotations.
 
@@ -16,9 +17,11 @@ Set Implicit Arguments.
 
 Parameter maxlen : addr. (* Number of entries on disk *)
 
+Definition kv_pointer := addr.
 Definition empty_value : valu := $0.
-Definition entry := (addr * valu)%type.
-Definition empty_entry : entry := ($0, $0).
+Definition empty_valuset : valuset := ($0, @nil valu).
+Definition entry := (valuset * valuset)%type.
+Definition empty_entry : entry := (empty_valuset, empty_valuset).
 
 Definition list_prefix A (p l : list A) :=
   firstn (length p) l = p.
@@ -32,57 +35,74 @@ Proof.
   lia.
 Qed.
 
-Definition rep l :=
-  (exists diskl,
-   $0 |-> addr2valu $ (length l) *
-   array $1 (map (fun e => addr2valu (fst e)) diskl) $2 *
+(* representation on memory? *)
+Definition rep l (kv_p : kv_pointer) xp st mscs := (exists diskl,
+  array $0 (map fst diskl) $2 *
+  array $1 (map snd diskl) $2 *
+  (* 2*len(diskl)? *)
+  [[ length diskl = wordToNat maxlen ]] *
+  [[ list_prefix l diskl ]] *
+  MEMLOG.rep xp st mscs)%pred.
+
+Definition rep' l (kv_p : kv_pointer) := (exists (diskl : list entry),
+  array $0 (map (fun e => fst (fst e)) diskl) $2 *
+  array $1 (map (fun e => fst (snd e)) diskl) $2 *
+  [[ length diskl = wordToNat maxlen ]] *
+  [[ list_prefix l diskl ]])%pred.
+
+
+(*
+Definition rep l := (exists diskl,
+   array $1  (kv_p : kv_pointer)(map (fun e => add
+  (*(weq (natToWord addrlen (length l)) kv_p) **)
+   $0 |-> addr2valu $ (length l) *r2valu (fst e)) diskl) $2 *
    array $2 (map snd diskl) $2 *
    [[ length diskl = wordToNat maxlen ]] *
    [[ list_prefix l diskl ]])%pred.
+*)
 
-Definition no_such_put (l : list entry) (k : addr) : Prop :=
-  ~ exists v, In (k, v) l.
+Definition no_such_put (l : list entry) (k : valu) : Prop :=
+  ~ exists v cs_k cs_v, In ((k, cs_k), (v, cs_v)) l.
 
-Fixpoint is_last_put (l : list entry) (k : addr) (v : valu) :=
+Fixpoint is_last_put (l : list entry) (k : valu) (v : valu) :=
   match l with
   | nil => False
   | (k', v') :: tl =>
-    (k = k' /\ v = v' /\ no_such_put l k) \/
+    (k = fst k' /\ v = fst v' /\ no_such_put l k) \/
     (is_last_put tl k v)
   end.
 
-Definition get T (k : addr) (rx : valu -> prog T) :=
-  l <- Read $0;
-  final_value <- For i < (valu2addr l)
-    Ghost on_disk_list
+Definition get T (kv_p : kv_pointer) key rx : prog T :=
+final_value <- For i < kv_p
     Loopvar current_value <- empty_value
     Continuation lrx
     Invariant
-      rep on_disk_list
+      any
     OnCrash
-      rep on_disk_list
+      any
     Begin
-      disk_key <- ArrayRead $1 i $2;
-      If (weq (valu2addr disk_key) k) {
-        disk_value <- ArrayRead $2 i $2;
+      disk_key <- Read i;
+      if (weq disk_key key) then
+        disk_value <- Read (i ^+ $1);
         lrx disk_value
-      } else {
+      else
         lrx current_value
-      }
   Rof;
-  rx final_value.
+rx final_value.
+
+Check rep nil.
 
 Hint Rewrite map_length.
 
-Theorem get_ok: forall k,
-  {< l,
-  PRE    rep l
-  POST:r rep l * [[ is_last_put l k r ]]
-  CRASH  rep l
-  >} get k.
-Proof.
-  unfold get, rep.
-  hoare.
+Theorem get_ok: forall kv_p k,
+  {< l xp st mscs,
+  PRE    rep l kv_p xp st mscs
+  POST:r rep l kv_p xp st mscs * [[ is_last_put l k r ]]
+  CRASH  rep l kv_p xp st mscs
+  >} get kv_p k.
+Pro kv_p xp st mscsof.
+  unfold ge kv_p xp st mscs * [[ is_last_put l k r ]]t, rep.
+  hoare kv_p xp st mscs.
 
   simpl_list.
   eapply lt_le_trans; [| apply list_prefix_length; eauto ].
@@ -99,6 +119,10 @@ Proof.
   admit.
 Qed.
 
+Definition put T (kv_p : kv_pointer) (key value : valu) rx : prog T :=
+  Write kv_p key;;
+  Write (kv_p ^+ $1) value;;
+  rx (kv_p ^+ $2).
 
 Definition put T k v (rx : bool -> prog T) :=
   l <- Read $0;
